holsrcs/concrete_testsScript.sml
@@ -32,6 +32,8 @@ val state1_def = Define`
 |>
 `;
 
+
+
 val simp = SIMP_CONV (srw_ss()) [state1_def]
 
 open environmentsTheory
@@ -72,6 +74,22 @@ val defined_classes = Store_thm(
 val cinfo_state1_c = Save_thm(
   "cinfo_state1_c",
   SIMP_CONV (srw_ss()) [cinfo_def] ``cinfo state1 cname``);
+
+val RTC_class_lt_cname = Store_thm(
+  "RTC_class_lt_cname",
+  ``state1 |- b <= cname = (b = cname)``,
+  SRW_TAC [][EQ_IMP_THM, RTC_class_lt_def, relationTheory.RTC_RULES] THEN
+  POP_ASSUM (MP_TAC o ONCE_REWRITE_RULE [relationTheory.RTC_CASES2]) THEN
+  SRW_TAC [][is_direct_base_def, get_direct_bases_def, is_virtual_base_def,
+             get_virtual_bases_def, relationTheory.RUNION]);
+
+val is_abstract_cname = Store_thm(
+  "is_abstract_cname",
+  ``is_abstract state1 cname = F``,
+  SRW_TAC [][is_abstract_def] THEN
+  Cases_on `bnm = cname` THEN SRW_TAC [][]);
+
+
 
 val nsdmembers_state1 = SIMP_CONV (srw_ss()) [nsdmembers_def]
                            ``nsdmembers state1 cname``
