holsrcs/declaration_dynamicsScript.sml
@@ -405,7 +405,7 @@ val (declmng_rules, declmng_ind, declmng_cases) = Hol_reln`
      object_type ty /\
      ~class_type (strip_array ty)
    ==>
-     declmng mng (VDec ty (IDConstant(F, [], name)), s0) ([], s))
+     declmng mng (VDec ty (IDConstant(F, [], SFName name)), s0) ([], s))
 
    /\
 
@@ -438,7 +438,7 @@ val (declmng_rules, declmng_ind, declmng_cases) = Hol_reln`
                                 base_se)))
                (array_size ty))
    ==>
-     declmng mng (VDec ty (IDConstant(F,[],name)), s0)
+     declmng mng (VDec ty (IDConstant(F,[],SFName name)), s0)
                  (subdecls, s))
 
    /\
@@ -463,7 +463,10 @@ val (declmng_rules, declmng_ind, declmng_cases) = Hol_reln`
      ((a,pth) = s1.varmap ' name)
    ==>
      declmng mng
-             (VDecInit ty (IDConstant(F,[],name)) (DirectInit0 args), s0)
+             (VDecInit ty
+                       (IDConstant(F,[],SFName name))
+                       (DirectInit0 args),
+              s0)
              ([VDecInitA ty
                          (ObjPlace a)
                          (DirectInit
@@ -513,7 +516,9 @@ val (declmng_rules, declmng_ind, declmng_cases) = Hol_reln`
      (loc = if ref_type ty then RefPlace NONE (Base name) else ObjPlace a)
    ==>
      declmng mng
-             (VDecInit ty (IDConstant(F,[],name)) (DirectInit0 [arg]), s0)
+             (VDecInit ty
+                       (IDConstant(F,[],SFName name))
+                       (DirectInit0 [arg]), s0)
              ([VDecInitA ty loc (CopyInit (mExpr arg base_se))], s))
 
    /\
@@ -525,7 +530,7 @@ val (declmng_rules, declmng_ind, declmng_cases) = Hol_reln`
      (loc = if ref_type ty then RefPlace NONE (Base name) else ObjPlace a)
    ==>
      declmng mng
-             (VDecInit ty (IDConstant(F,[],name)) (CopyInit arg), s0)
+             (VDecInit ty (IDConstant(F,[],SFName name)) (CopyInit arg), s0)
              ([VDecInitA ty loc (CopyInit arg)], s))
 
    /\
