holsrcs/environmentsScript.sml
@@ -52,7 +52,7 @@ val _ = type_abbrev("state_class_info",
 
 
 val _ = type_abbrev("construction_locn",
-                    ``:addr # class_spec # class_spec list``)
+                    ``:addr # CPP_ID # CPP_ID list``)
 
 val _ = Hol_datatype`
   class_envinfo = <|
@@ -70,7 +70,7 @@ val _ = Hol_datatype`
   envinfo = <| varmap   : string |-> addr # CPP_ID list ;
                typemap  : StaticField |-> CPP_Type ;
                classenv : StaticField |-> class_env ;
-               funs     : StaticField |-> CPP_ID (* function's fullname *)
+               nspaces : string set (* as opposed to a class *)
 |>`;
 
 (* strings are the keys here, because these are ever-deepening
@@ -80,8 +80,7 @@ val _ = type_abbrev ("environment", ``:(string,envinfo)fmaptree``)
 val empty_env_def = Define`
   empty_env = FTNode <| varmap := FEMPTY ;
                         typemap := FEMPTY ;
-                        classenv := FEMPTY ;
-                        funs := FEMPTY |>
+                        classenv := FEMPTY |>
                      FEMPTY
 `;
 
@@ -90,31 +89,33 @@ val lookup_nspace_def = Define`
   (lookup_nspace env (h::t) = lookup_nspace (map env ' h) t)
 `;
 
-val elookup_class_def = Define`
-  (elookup_class env (IDFld id fld) =
-     case elookup_class env id of
+val celookup_class_def = Define`
+  (celookup_class cenv (IDConstant(b, [], sf)) = FLOOKUP cenv sf) /\
+  (celookup_class cenv (IDConstant(b, h :: t, sf)) =
+     case FLOOKUP cenv h of
         NONE -> NONE
-     || SOME cenv -> FLOOKUP (map cenv) fld) /\
-  (elookup_class env (IDConstant (b, [], n)) =
-      FLOOKUP ((item env).classenv) (SFName n)) /\
-  (elookup_class env (IDConstant (b, h :: t, n)) =
-      case FLOOKUP (map env) h of
-         NONE -> NONE
-      || SOME m -> elookup_class m (IDConstant(b, t, n))) /\
-  (elookup_class env (IDTempCall (TemplateConstant (b, [], n)) targs) =
-      FLOOKUP ((item env).classenv) (SFTempCall n targs)) /\
-  (elookup_class env (IDTempCall (TemplateConstant (b, h::t, n)) targs) =
-      case FLOOKUP (map env) h of
-         NONE -> NONE
-      || SOME m -> elookup_class m
-                         (IDTempCall (TemplateConstant (b, t, n)) targs)) /\
-  (elookup_class env _ = NONE)
+     || SOME cei -> celookup_class (map cei) (IDConstant(b, t, sf))) /\
+  (celookup_class cenv _ = NONE)
+`;
+
+val elookup_class_def = Define`
+  (elookup_class env (IDConstant (b, [], sf)) =
+     FLOOKUP ((item env).classenv) sf) /\
+  (elookup_class env (IDConstant (b, SFName h :: t, sf)) =
+      if SFName h IN FDOM (item env).classenv then
+        celookup_class (item env).classenv (IDConstant(b, SFName h :: t, sf))
+      else
+        case FLOOKUP (map env) h of
+           NONE -> NONE
+        || SOME e' -> elookup_class e' (IDConstant(b, t, sf))) /\
+  (elookup_class env (IDConstant(b, sfs, sf2)) =
+      celookup_class (item env).classenv (IDConstant(b, sfs, sf2))) /\
+  (elookup_class _ _ = NONE)
 `;
 
 val is_class_name_env_def = Define`
   (is_class_name_env env id = ?c. elookup_class env id = SOME c)
 `;
-
 
 val update_classenv_def = Define`
   (update_classenv [] i (cenv : StaticField |-> class_env) = NONE) /\
@@ -131,91 +132,15 @@ val update_classenv_def = Define`
      else NONE)
 `;
 
+(* class id has no namespace constituents - i.e., this is OK for a local
+   class, but not OK for a top-level declaration... *)
 val update_class_def = Define`
-  update_class id i env =
-     let (bid, sfs) = strip_field id
-     in
-       case strip_nspaces bid of
-          NONE -> NONE
-       || SOME ((b, ns), sf) ->
-            fupd_at_path ns
-              (\ft. case update_classenv (sf::sfs) i (item ft).classenv of
-                       NONE -> NONE
-                    || SOME ce' -> SOME (FTNode (item ft with classenv := ce')
-                                                (map ft)))
-              env
-`
-
-
-val id_GSPEC_cases = store_thm(
-  "id_GSPEC_cases",
-  ``{ id | P id } =
-      { IDVar s | P (IDVar s) } UNION
-      { IDFld id sf | P (IDFld id sf) } UNION
-      { IDTempCall tid targs | P (IDTempCall tid targs) } UNION
-      { IDConstant tn | P (IDConstant tn) }``,
-  SRW_TAC [][EXTENSION] THEN Cases_on `x` THEN SRW_TAC [][]);
-
-val option_case_lemma = prove(
-  ``(option_case NONE f x = SOME y) = ?z. (x = SOME z) /\ (f z = SOME y)``,
-  Cases_on `x` THEN SRW_TAC [][]);
-
-(* SANITY *)
-(* empty list is an error case *)
-val class_part_def = Define`
-  (class_part (IDFld id fld) =
-     case class_part id of
-        [] -> []
-     || list -> list ++ [fld]) /\
-  (class_part (IDConstant(b,l,n)) = [SFName n]) /\
-  (class_part (IDTempCall (TemplateConstant(b,l,n)) targs) =
-              [SFTempCall n targs]) /\
-  (class_part _ = [])
+  update_class (IDConstant(b, sfs, sf)) i env =
+     case update_classenv (sfs ++ [sf]) i (item env).classenv of
+        NONE -> NONE
+     || SOME ce' -> SOME (FTNode (item env with classenv := ce')
+                                 (map env))
 `;
-
-val option_case_lemma2 = prove(
-  ``option_case NONE (\x. SOME x) y = y``,
-  Cases_on `y` THEN SRW_TAC [][]);
-
-val list_case_lemma = prove(
-  ``(list_case NONE f x = SOME y) =
-    ?h t. (x = h :: t) /\ (f h t = SOME y)``,
-  Cases_on `x` THEN SRW_TAC [][]);
-
-val elookup_class_apply_path = store_thm(
-  "elookup_class_apply_path",
-  ``!env id.
-       elookup_class env id =
-          case class_part id of
-             [] -> NONE
-          || h::t -> (case apply_path (SND (id_namespaces id)) env of
-                         NONE -> NONE
-                      || SOME e -> (case FLOOKUP (item e).classenv h of
-                                       NONE -> NONE
-                                    || SOME ce -> apply_path t ce))``,
-  HO_MATCH_MP_TAC (theorem "elookup_class_ind") THEN
-  SRW_TAC [][elookup_class_def, fmaptreeTheory.apply_path_def, class_part_def,
-             typesTheory.id_namespaces_def, typesTheory.tid_namespaces_def,
-             option_case_lemma2] THEN
-  TRY (SRW_TAC [][finite_mapTheory.FLOOKUP_DEF] THEN NO_TAC) THEN
-  Cases_on `class_part id` THEN SRW_TAC [][] THEN
-  Cases_on `apply_path (SND (id_namespaces id)) env` THEN SRW_TAC [][] THEN
-  Cases_on `FLOOKUP (item x).classenv h` THEN SRW_TAC [][] THEN
-  SRW_TAC [][fmaptreeTheory.apply_path_SNOC]);
-
-(* tricksy
-val env_classes_FINITE = store_thm(
-  "env_classes_FINITE",
-  ``!env. FINITE { id | is_class_name_env env id }``,
-  SIMP_TAC (srw_ss()) [is_class_name_env_def] THEN
-  SRW_TAC [DNF_ss][elookup_class_apply_path, option_case_lemma,
-                   list_case_lemma] THENL [
-    Q_TAC SUFF_TAC `{IDVar s | F} = {}` THEN1 SRW_TAC [][] THEN
-    SRW_TAC [][EXTENSION],
-    SRW_TAC [][option_case_lemma]
-*)
-
-
 
 
 val _ = export_theory()
